trying to reformulate value invs

examples/wysteria/ast.fst
@@ -32,47 +32,57 @@ type const =
   | C_bool : c:bool -> const
 
 type exp' =
-  | E_aspar: ps:exp -> e:exp -> exp'
-  | E_assec: ps:exp -> e:exp -> exp'
-  | E_unbox: e:exp  -> exp'
+  | E_aspar : ps:exp -> e:exp -> exp'
+  | E_assec : ps:exp -> e:exp -> exp'
+  | E_unbox : e:exp  -> exp'
 
-  | E_const: c:const -> exp'
-  | E_var  : x:varname -> exp'
-  | E_let  : x:varname -> e1:exp -> e2:exp -> exp'
-  | E_abs  : x:varname -> e:exp -> exp'
-  | E_app  : e1:exp -> e2:exp -> exp'
+  | E_const : c:const -> exp'
+  | E_var   : x:varname -> exp'
+  | E_let   : x:varname -> e1:exp -> e2:exp -> exp'
+  | E_abs   : x:varname -> e:exp -> exp'
+  | E_empabs: x:varname -> e:exp -> exp'
+  | E_app   : e1:exp -> e2:exp -> exp'
 
 and exp =
   | Exp: e:exp' -> info:option other_info -> exp
 
-type value: eprins -> Type =
-  | V_const  : c:const -> value empty
-  | V_box    : #vps:eprins -> ps:prins -> v:value vps{subset vps ps}
-               -> value ps
-  | V_clos   : en:env -> x:varname -> e:exp -> value empty
+type canbox = | Can_b | Cannot_b
+
+type v_meta = eprins * canbox
+
+type value: v_meta -> Type =
+  | V_const   : c:const -> value (empty, Can_b)
+
+  | V_box     : #meta:v_meta -> ps:prins
+                -> v:value meta{subset (fst meta) ps /\ (snd meta) = Can_b}
+                -> value (ps, Can_b)
+
+  | V_clos    : en:env -> x:varname -> e:exp -> value (empty, Cannot_b)
+  
+  | V_emp_clos: x:varname -> e:exp -> value (empty, Can_b)
 
   (* bomb value, comes up in target only *)
-  | V_emp    : value empty
+  | V_emp     : value (empty, Can_b)
 
 and dvalue:Type =
-  | DV: vps:eprins -> v:value vps -> dvalue
+  | D_v: meta:v_meta -> v:value meta -> dvalue
 
-(* TODO: fix it, option value *)
-and env = varname -> Tot dvalue
+and env = varname -> Tot (option dvalue)
 
 type redex =
-  | R_aspar: #vps:eprins -> ps:prins -> v:value vps -> redex
-  | R_assec: #vps:eprins -> ps:prins -> v:value vps -> redex
-  | R_box  : #vps:eprins -> ps:prins -> v:value vps -> redex
-  | R_unbox: #vps:eprins -> v:value vps -> redex
-  | R_let  : #vps:eprins -> x:varname -> v:value vps -> e:exp -> redex
-  | R_app  : #vps1:eprins -> #vps2:eprins -> v1:value vps1 -> v2:value vps2
+  | R_aspar: #meta:v_meta -> ps:prins -> v:value meta -> redex
+  | R_assec: #meta:v_meta -> ps:prins -> v:value meta -> redex
+  | R_box  : #meta:v_meta -> ps:prins -> v:value meta -> redex
+  | R_unbox: #meta:v_meta -> v:value meta -> redex
+  | R_let  : #meta:v_meta -> x:varname -> v:value meta -> e:exp -> redex
+  | R_app  : #meta1:v_meta -> #meta2:v_meta -> v1:value meta1 -> v2:value meta2
              -> redex
 
-assume val empty_env: env
+val empty_env: env
+let empty_env = fun _ -> None
 
-val update_env: #vps:eprins -> env -> varname -> value vps -> Tot env
-let update_env #vps en x v = fun y -> if y = x then DV vps v else en y
+val update_env: #meta:v_meta -> env -> varname -> value meta -> Tot env
+let update_env #meta en x v = fun y -> if y = x then Some (D_v meta v) else en y
 
 type as_mode =
   | Par
@@ -91,7 +101,7 @@ type frame' =
   | F_unbox    : frame'
   | F_let      : x:varname -> e2:exp -> frame'
   | F_app_e1   : e2:exp -> frame'
-  | F_app_e2   : #vps:eprins -> v:value vps -> frame'
+  | F_app_e2   : #meta:v_meta -> v:value meta -> frame'
   
 type frame =
   | Frame: m:mode -> en:env -> f:frame'-> frame
@@ -101,7 +111,7 @@ type stack = list frame
 type term =
   | T_exp     : e:exp -> term
   | T_red     : r:redex -> term
-  | T_val     : #vps:eprins -> v:value vps -> term
+  | T_val     : #meta:v_meta -> v:value meta -> term
   
   | T_sec_wait: term
 
@@ -168,8 +178,8 @@ let is_value_ps c = match c with
   | Conf _ _ _ _ (T_val (V_const (C_prins _))) -> true
   | _                                          -> false
 
-val c_value: c:config{is_value c} -> Tot (vps:eprins & value vps)
-let c_value (Conf _ _ _ _ (T_val #vps v)) = (| vps, v |)
+val c_value: c:config{is_value c} -> Tot dvalue
+let c_value (Conf _ _ _ _ (T_val #meta v)) = D_v meta v
 
 val c_value_ps: c:config{is_value_ps c} -> Tot prins
 let c_value_ps c = match c with
@@ -190,11 +200,15 @@ type pre_eapp (c:config) =
 type pre_eabs (c:config) =
   is_T_exp (Conf.t c) /\ is_E_abs (Exp.e (T_exp.e (Conf.t c)))
 
+type pre_eempabs (c:config) =
+  is_T_exp (Conf.t c) /\ is_E_empabs (Exp.e (T_exp.e (Conf.t c)))
+
 type pre_elet (c:config) =
   is_T_exp (Conf.t c) /\ is_E_let (Exp.e (T_exp.e (Conf.t c)))
 
 type pre_evar (c:config) =
-  is_T_exp (Conf.t c) /\ is_E_var (Exp.e (T_exp.e (Conf.t c)))
+  is_T_exp (Conf.t c) /\ is_E_var (Exp.e (T_exp.e (Conf.t c))) /\
+  is_Some ((Conf.en c) (E_var.x (Exp.e (T_exp.e (Conf.t c)))))
 
 type pre_econst (c:config) =
   is_T_exp (Conf.t c) /\ is_E_const (Exp.e (T_exp.e (Conf.t c)))
@@ -219,7 +233,7 @@ let step_const (Conf l m s en (T_exp (Exp (E_const c) _))) =
 
 val step_var: c:config{pre_evar c} -> Tot config
 let step_var (Conf l m s en (T_exp (Exp (E_var x) _))) =
-  let DV _ v = en x in
+  let Some (D_v _ v) = en x in
   Conf l m s en (T_val v)
 
 val step_let_e1: c:config{pre_elet c} -> Tot config
@@ -229,6 +243,10 @@ let step_let_e1 (Conf l m s en (T_exp (Exp (E_let x e1 e2) _))) =
 val step_abs: c:config{pre_eabs c} -> Tot config
 let step_abs (Conf l m s en (T_exp (Exp (E_abs x e) _))) =
   Conf l m s en (T_val (V_clos en x e))
+
+val step_empabs: c:config{pre_eempabs c} -> Tot config
+let step_empabs (Conf l m s en (T_exp (Exp (E_empabs x e) _))) =
+  Conf l m s en (T_val (V_emp_clos x e))
 
 val step_app_e1: c:config{pre_eapp c} -> Tot config
 let step_app_e1 (Conf l m s en (T_exp (Exp (E_app e1 e2) _))) =
@@ -270,19 +288,30 @@ val step_app_red: c:config{is_value c /\ is_sframe c is_F_app_e2}
 let step_app_red (Conf l _ ((Frame m en (F_app_e2 v1))::s) _ (T_val v2)) =
   Conf l m s en (T_red (R_app v1 v2))
 
+val is_clos: #meta:v_meta -> value meta -> Tot bool
+let is_clos #meta v = is_V_clos v || is_V_emp_clos v
+
+val get_en_b: #meta:v_meta -> v:value meta{is_clos v} -> Tot (env * varname * exp)
+let get_en_b #meta v = match v with
+  | V_clos en x e  -> en, x, e
+  | V_emp_clos x e -> empty_env, x, e
+
 val pre_aspar: config -> Tot comp
 let pre_aspar c = match c with
-  | Conf l (Mode Par ps1) _ _ (T_red (R_aspar ps2 (V_clos _ _ _))) ->
-    if src l then
-      if subset ps2 ps1 then Do else NA
-    else
-      if subset ps1 ps2 then Do else Skip
+  | Conf l (Mode Par ps1) _ _ (T_red (R_aspar ps2 v)) ->
+    if is_clos v then
+      if src l then
+        if subset ps2 ps1 then Do else NA
+      else
+        if subset ps1 ps2 then Do else Skip
+    else NA
   
   | _ -> NA
 
 val step_aspar: c:config{not (pre_aspar c = NA)} -> Tot config
 let step_aspar c = match c with
-  | Conf l m s en' (T_red (R_aspar ps (V_clos en x e))) ->
+  | Conf l m s en' (T_red (R_aspar ps v)) ->
+    let en, x, e = get_en_b v in
     let m'  = if src l then Mode Par ps else m in
     let s'  = (Frame m en' (F_box_e ps))::s in
     
@@ -302,8 +331,9 @@ let step_aspar c = match c with
 
 val pre_box: config -> Tot comp
 let pre_box c = match c with
-  | Conf l (Mode Par ps1) _ _ (T_red (R_box #vps ps2 _)) ->
-    if subset vps ps2 then
+  | Conf l (Mode Par ps1) _ _ (T_red (R_box #meta ps2 _)) ->
+    let (ps', b) = meta in
+    if subset ps' ps2 && is_Can_b b then
       if src l then
         if subset ps2 ps1 then Do else NA
       else Do
@@ -322,7 +352,6 @@ let pre_unbox c = match c with
       if subset ps1 ps2 then Do else NA
     else
       if not (intersect ps1 ps2 = empty) then Do else NA
-      (*if subset ps2 ps1 then Do else NA*)
 
   | _ -> NA
 
@@ -342,13 +371,14 @@ let step_let c = match c with
 
 val is_app_redex: c:config -> Tot bool
 let is_app_redex c = match c with
-  | Conf _ _ _ _ (T_red (R_app (V_clos _ _ _) _)) -> true
+  | Conf _ _ _ _ (T_red (R_app v _)) -> is_clos v
 
   | _ -> false
 
 val step_app: c:config{is_app_redex c} -> Tot config
 let step_app c = match c with
-  | Conf l m s _ (T_red (R_app (V_clos en x e) v)) ->
+  | Conf l m s _ (T_red (R_app f v)) ->
+    let (en, x, e) = get_en_b f in
     Conf l m s (update_env en x v) (T_exp e)
 
 type cstep: config -> config -> Type =
@@ -375,6 +405,10 @@ type cstep: config -> config -> Type =
 
   | C_abs:
     c:config{pre_eabs c} -> c':config{c' = step_abs c}
+    -> cstep c c'
+  
+  | C_empabs:
+    c:config{pre_eempabs c} -> c':config{c' = step_empabs c}
     -> cstep c c'
 
   | C_app_e1:
@@ -455,16 +489,19 @@ let step_assec_red (Conf l _ ((Frame m en (F_assec_e ps))::s) _ (T_val v)) =
 
 val pre_assec: config -> Tot comp
 let pre_assec c = match c with
-  | Conf l (Mode as_m ps1) _ _ (T_red (R_assec ps2 (V_clos _ _ _))) ->
-    if l = Source || as_m = Sec then
-      if ps1 = ps2 then Do else NA
+  | Conf l (Mode as_m ps1) _ _ (T_red (R_assec ps2 v)) ->
+    if is_clos v then
+      if l = Source || as_m = Sec then
+        if ps1 = ps2 then Do else NA
+      else NA
     else NA
 
   | _ -> NA
 
 val step_assec: c:config{not (pre_assec c = NA)} -> Tot config
 let step_assec c = match c with
-  | Conf l m s en' (T_red (R_assec ps (V_clos en x e))) ->  
+  | Conf l m s en' (T_red (R_assec ps v)) ->
+    let (en, x, e) = get_en_b v in
     Conf l (Mode Sec ps) ((Frame m en' F_assec_ret)::s)
            (update_env en x (V_const C_unit)) (T_exp e)
 
@@ -502,68 +539,145 @@ type sstep: config -> config -> Type =
 
 (**********)
 
-
 assume val preceds_axiom: en:env -> x:varname -> Lemma (ensures (en x << en))
 
-val slice_v : #vps:eprins -> prin -> v:value vps -> Tot (r:dvalue{subset (DV.vps r) vps}) (decreases %[v])
-val slice_en: prin -> en:env -> Tot (varname -> Tot dvalue) (decreases %[en])
+type slice_v_meta_inv (meta:v_meta) (smeta:v_meta) =
+  subset (fst smeta) (fst meta) && (snd smeta = snd meta)
 
-let rec slice_v #vps p v =
+val slice_v : #meta:v_meta -> prin -> v:value meta
+              -> Tot (r:dvalue{slice_v_meta_inv meta (D_v.meta r)}) (decreases %[v])
+val slice_en: prin -> en:env -> Tot (varname -> Tot (option dvalue)) (decreases %[en])
+
+let rec slice_v #meta p v =
+  let def = D_v meta v in
+  let emp = D_v (empty, Can_b) V_emp in
   match v with
-    | V_const _     -> DV vps v
-    | V_box ps v'   ->
-      let DV _ v'' = if mem p ps then slice_v p v' else DV empty V_emp in
-      DV ps (V_box ps v'')
-    | V_clos en x e -> DV empty (V_clos (slice_en p en) x e)
-    | V_emp         -> DV vps v
+    | V_const _      -> def
+  
+    | V_box ps v     ->
+      let D_v _ v' = if mem p ps then slice_v p v else emp in
+      D_v meta (V_box ps v')
+
+    | V_clos en x e  -> D_v meta (V_clos (slice_en p en) x e)
+    
+    | V_emp_clos _ _ -> def
+
+    | V_emp          -> emp
 
 and slice_en p en =
   let _ = () in
-  fun x -> preceds_axiom en x; slice_v p (DV.v (en x))
+  fun x -> preceds_axiom en x;
+           if en x = None then None
+           else
+             Some (slice_v p (D_v.v (Some.v (en x))))
 
-assume val slice_emp_en: p:prin
-                         -> Lemma (requires (True))
-                                  (ensures (slice_en p empty_env = empty_env))
-                            [SMTPat (slice_en p empty_env)]
+open FunctionalExtensionality
+
+val slice_emp_en: p:prin
+                  -> Lemma (requires (True))
+                           (ensures (slice_en p empty_env = empty_env))
+                     [SMTPat (slice_en p empty_env)]
+let slice_emp_en p =
+  let _ = cut (FEq (slice_en p empty_env) empty_env) in
+  ()
 
 
-val compose_vals: #vps1:eprins -> #vps2:eprins -> v1:value vps1 -> v2:value vps2
-                  -> Tot (r:dvalue{subset (DV.vps r) (union vps1 vps2)})
+type compose_v_meta_inv (m1:v_meta) (m2:v_meta) (cmeta:v_meta) =
+  subset (fst cmeta) (union (fst m1) (fst m2)) /\
+  ((snd m1 = Can_b /\ snd m2 = Can_b) ==> snd cmeta = Can_b)
+
+val compose_vals: #m1:v_meta -> #m2:v_meta -> v1:value m1 -> v2:value m2
+                  -> Tot (r:dvalue{compose_v_meta_inv m1 m2 (D_v.meta r)})
                      (decreases %[v1])
-val compose_envs: en:env -> env -> Tot (varname -> Tot dvalue) (decreases %[en])
+val compose_envs: en:env -> env -> Tot (varname -> Tot (option dvalue)) (decreases %[en])
 
-let rec compose_vals #vps1 #vps2 v1 v2 =
-  let def = DV empty V_emp in
+let rec compose_vals #m1 #m2 v1 v2 =
+  let emp = D_v (empty, Can_b) V_emp in
   match v1 with
     | V_const c1 ->
       if is_V_const v2 && V_const.c v1 = V_const.c v2 then
-        DV vps1 v1
-      else def
+        D_v m1 v1
+      else emp
       
-    | V_box ps1 v1' ->
+    | V_box ps1 v1 ->
       if is_V_box v2 then
-        let V_box ps2 v2' = v2 in
+        let V_box ps2 v2 = v2 in
         if ps1 = ps2 then
-          DV ps1 (V_box ps1 (DV.v (compose_vals v1' v2')))
+          D_v m1 (V_box ps1 (D_v.v (compose_vals v1 v2)))
         else
-          def
-      else def
+          emp
+      else emp
       
     | V_clos en1 x1 e1 ->
       if is_V_clos v2 then
         let V_clos en2 x2 e2 = v2 in
         if x1 = x2 && e1 = e2 then
-          DV vps1 (V_clos (compose_envs en1 en2) x1 e1)
-        else def
-      else def
+          D_v m1 (V_clos (compose_envs en1 en2) x1 e1)
+        else emp
+      else emp
       
-    | V_emp -> DV vps2 v2
+    | V_emp_clos x1 e1 ->
+      if is_V_emp_clos v2 then
+        let V_emp_clos x2 e2 = v2 in
+        if x1 = x2 && e1 = e2 then
+          D_v m1 (V_emp_clos x1 e1)
+        else emp
+      else emp
+      
+    | V_emp -> D_v m2 v2
     
-    | _ -> if is_V_emp v2 then DV vps1 v1 else def
+    | _ -> if is_V_emp v2 then D_v m1 v1 else emp
       
 and compose_envs en1 en2 =
   let _ = () in
-  fun x -> preceds_axiom en1 x; compose_vals (DV.v (en1 x)) (DV.v (en2 x))
+  fun x -> preceds_axiom en1 x;
+           let r1 = en1 x in
+           let r2 = en2 x in
+           match r1 with
+             | None             -> r2
+             | Some (D_v m1 v1) ->
+               match r2 with
+                 | None             -> r1
+                 | Some (D_v m2 v2) -> Some (compose_vals v1 v2)
+
+val slice_v_sps : #meta:v_meta -> prins -> v:value meta
+                  -> Tot (r:dvalue{slice_v_meta_inv meta (D_v.meta r)}) (decreases %[v])
+val slice_en_sps: prins -> en:env -> Tot (varname -> Tot (option dvalue)) (decreases %[en])
+
+let rec slice_v_sps #meta ps v =
+  let def = D_v meta v in
+  let emp = D_v (empty, Can_b) V_emp in
+  match v with
+   | V_const _      -> def
+   
+   | V_box ps' v    ->
+     let D_v _ v' =
+       //let ps'' = intersect ps' ps in
+       if intersect ps' ps = empty then emp
+       else slice_v_sps ps v
+     in
+     D_v meta (V_box ps' v')
+
+   | V_clos en x e  -> D_v meta (V_clos (slice_en_sps ps en) x e)
+   
+   | V_emp_clos _ _ -> def
+
+   | V_emp          -> emp
+
+and slice_en_sps ps en =
+ let _ = () in
+ fun x -> preceds_axiom en x;
+          if en x = None then None
+          else
+            Some (slice_v_sps ps (D_v.v (Some.v (en x))))
+
+val slice_emp_en_sps: ps:prins
+                      -> Lemma (requires (True))
+                               (ensures (slice_en_sps ps empty_env = empty_env))
+                         [SMTPat (slice_en_sps ps empty_env)]
+let slice_emp_en_sps ps =
+  let _ = cut (FEq (slice_en_sps ps empty_env) empty_env) in
+  ()
 
 
 (*type value_map = OrdMap.ordmap prin value p_cmp
@@ -584,7 +698,7 @@ let mremove (#k:Type) (#v:Type) #f = OrdMap.remove #k #v #f
 let mchoose (#k:Type) (#v:Type) #f = OrdMap.choose #k #v #f
 let msize (#k:Type) (#v:Type) #f = OrdMap.size #k #v #f
 
-val slice_v_ps: #vps:eprins -> prins -> v:value vps -> Tot (value_map)*)
+val slice_v_ps: #meta:v_meta -> prins -> v:valuemeta -> Tot (value_map)*)
 
 (*val compose_vals_m: m:value_map{not (m = mempty)} -> Tot value (decreases (msize m))
 let rec compose_vals_m m =
@@ -618,25 +732,25 @@ val
 
 
 
-val slice_v_sps : #vps:eprins -> prins -> v:value vps -> Tot (r:dvalue{subset (DV.vps r) vps})  (decreases %[v])
+val slice_v_sps : #meta:v_meta -> prins -> v:valuemeta -> Tot (r:dvalue{subset (D_vmeta r)#meta})  (decreases %[v])
 val slice_en_sps: prins -> en:env -> Tot (varname -> Tot dvalue) (decreases %[en])
 
-let rec slice_v_sps #vps ps v =
+let rec slice_v_sps #meta ps v =
   match v with
-    | V_const _     -> DV vps v
+    | V_const _     -> D_vmeta v
     | V_box ps' v'  ->
-      let DV _ v'' =
+      let D_v _ v'' =
         let ps'' = intersect ps' ps in
         if not (ps'' = empty) then slice_v_sps ps'' v'
-        else DV empty V_emp
+        else D_v empty V_emp
       in
-      DV ps' (V_box ps' v'')
-    | V_clos en x e -> DV empty (V_clos (slice_en_sps ps en) x e)
-    | V_emp         -> DV vps v
+      D_v ps' (V_box ps' v'')
+    | V_clos en x e -> D_v empty (V_clos (slice_en_sps ps en) x e)
+    | V_emp         -> D_vmeta v
 
 and slice_en_sps ps en =
   let _ = () in
-  fun x -> preceds_axiom en x; slice_v_sps ps (DV.v (en x))
+  fun x -> preceds_axiom en x; slice_v_sps ps (D_v.v (en x))
 
 assume val slice_emp_en_sps: ps:prins
                              -> Lemma (requires (True))
@@ -648,10 +762,10 @@ let slice_e_sps ps e = e
 
 val slice_r_sps: prins -> r:redex{is_sec_redex r} -> Tot redex
 let slice_r_sps ps r = match r with
-  | R_assec ps' v  -> R_assec ps' (DV.v (slice_v_sps ps v))
-  | R_unbox v     -> R_unbox (DV.v (slice_v_sps ps v))
-  | R_let x v1 e2 -> R_let x (DV.v (slice_v_sps ps v1)) e2
-  | R_app v1 v2   -> R_app (DV.v (slice_v_sps ps v1)) (DV.v (slice_v_sps ps v2))
+  | R_assec ps' v  -> R_assec ps' (D_v.v (slice_v_sps ps v))
+  | R_unbox v     -> R_unbox (D_v.v (slice_v_sps ps v))
+  | R_let x v1 e2 -> R_let x (D_v.v (slice_v_sps ps v1)) e2
+  | R_app v1 v2   -> R_app (D_v.v (slice_v_sps ps v1)) (D_v.v (slice_v_sps ps v2))
 
 val slice_f'_sps: ps:prins -> f:frame'{is_sec_frame f} -> Tot frame'
 let slice_f'_sps ps f = match f with
@@ -661,7 +775,7 @@ let slice_f'_sps ps f = match f with
   | F_unbox      -> f
   | F_let    _ _ -> f
   | F_app_e1   _ -> f
-  | F_app_e2   v -> F_app_e2  (DV.v (slice_v_sps ps v))
+  | F_app_e2   v -> F_app_e2  (D_v.v (slice_v_sps ps v))
 
 val slice_f_sps: ps:prins -> f:frame{Frame.m f = Mode Sec ps /\
                                      is_sec_frame (Frame.f f)}
@@ -683,7 +797,7 @@ val slice_t_sps: ps:prins -> t:term{term_inv t (Mode Sec ps) Source} -> Tot term
 let slice_t_sps ps t = match t with
   | T_exp _ -> t
   | T_red r -> T_red (slice_r_sps ps r)
-  | T_val v -> T_val (DV.v (slice_v_sps ps v))
+  | T_val v -> T_val (D_v.v (slice_v_sps ps v))
 
 val slice_c_sps: c:sconfig{is_sec c} -> Tot tconfig
 let slice_c_sps (Conf _ (Mode Sec ps) s en t) =
@@ -696,14 +810,14 @@ open Constructive
 
 open FunctionalExtensionality
 
-val env_upd_slice_lemma_ps: #vps:eprins -> ps:prins -> en:env -> x:varname -> v:value vps
+val env_upd_slice_lemma_ps: #meta:v_meta -> ps:prins -> en:env -> x:varname -> v:valuemeta
                             -> Lemma (requires (True))
                                      (ensures (slice_en_sps ps (update_env en x v) =
-                                               update_env (slice_en_sps ps en) x (DV.v (slice_v_sps ps v))))
+                                               update_env (slice_en_sps ps en) x (D_v.v (slice_v_sps ps v))))
                                      [SMTPat (slice_en_sps ps (update_env en x v))]
-let env_upd_slice_lemma_ps #vps ps en x v =
+let env_upd_slice_lemma_ps #meta ps en x v =
   cut (FEq (slice_en_sps ps (update_env en x v))
-      (update_env (slice_en_sps ps en) x (DV.v (slice_v_sps ps v))))
+      (update_env (slice_en_sps ps en) x (D_v.v (slice_v_sps ps v))))
 
 val cstep_sec_slice_lemma: c:sconfig{is_sec c} -> c':sconfig -> h:cstep c c'
                            -> Tot (cand (u:unit{Conf.m c' = Conf.m c})
@@ -754,14 +868,14 @@ let slice_e p e = e
 
 val slice_r: prin -> redex -> Tot redex
 let slice_r p r = match r with
-  | R_aspar ps v  -> R_aspar ps (DV.v (slice_v p v))
-  | R_assec ps v  -> R_assec ps (DV.v (slice_v p v))
+  | R_aspar ps v  -> R_aspar ps (D_v.v (slice_v p v))
+  | R_assec ps v  -> R_assec ps (D_v.v (slice_v p v))
   | R_box ps v    ->
-    let DV _ v' = if mem p ps then slice_v p v else DV empty V_emp in
+    let D_v _ v' = if mem p ps then slice_v p v else D_v empty V_emp in
     R_box ps v'
-  | R_unbox v     -> R_unbox (DV.v (slice_v p v))
-  | R_let x v1 e2 -> R_let x (DV.v (slice_v p v1)) e2
-  | R_app v1 v2   -> R_app (DV.v (slice_v p v1)) (DV.v (slice_v p v2))
+  | R_unbox v     -> R_unbox (D_v.v (slice_v p v))
+  | R_let x v1 e2 -> R_let x (D_v.v (slice_v p v1)) e2
+  | R_app v1 v2   -> R_app (D_v.v (slice_v p v1)) (D_v.v (slice_v p v2))
 
 val slice_f': p:prin -> f:frame'{not (is_F_assec_ret f)} -> Tot frame'
 let slice_f' p f = match f with
@@ -773,7 +887,7 @@ let slice_f' p f = match f with
   | F_unbox      -> f
   | F_let    _ _ -> f
   | F_app_e1   _ -> f
-  | F_app_e2   v -> F_app_e2  (DV.v (slice_v p v))
+  | F_app_e2   v -> F_app_e2  (D_v.v (slice_v p v))
 
 val slice_f: p:prin -> f:frame{Mode.m (Frame.m f) = Par    /\
                                mem p (Mode.ps (Frame.m f)) /\
@@ -797,7 +911,7 @@ let rec slice_s p s = match s with
 
 val slice_t: p:prin -> t:term{not (t = T_sec_wait)} -> Tot term
 let slice_t p t = match t with
-  | T_val v -> T_val (DV.v (slice_v p v))
+  | T_val v -> T_val (D_v.v (slice_v p v))
   | T_exp e -> t
   | T_red r -> T_red (slice_r p r)
 
@@ -819,18 +933,18 @@ let rec slice_c p (Conf Source (Mode as_m ps) s en t) =
 (**********)
 
 
-(*val slice_weakening: #vps:eprins -> v:value vps -> ps:prins
-                     -> ps':prins{intersect ps' vps = empty}
+(*val slice_weakening: #meta:v_meta -> v:valuemeta -> ps:prins
+                     -> ps':prins{intersect ps'#meta = empty}
                      -> Lemma (requires (True))
                               (ensures (slice_v_sps ps v = slice_v_sps (union ps ps') v))
                         (decreases %[v])
 val slice_weakening_en: en:env -> ps:prins
-                        -> ps':prins{intersect ps' vps = empty}
+                        -> ps':prins{intersect ps'#meta = empty}
                         -> Lemma (requires (True))
                               (ensures (slice_en_sps ps en = slice_en_sps (union ps ps') v))
                            (decreases %[en])
 
-let rec slice_weakening #vps v ps ps' = match v with
+let rec slice_weakening #meta v ps ps' = match v with
   | V_const _ -> ()
   
   | V_box ps'' v'' ->
